Fixed semantic def

lean/incorrectness_logic.lean
@@ -20,57 +20,72 @@ inductive LogicType : Type
 | er
 | ok
 
-inductive post: IncLoLang.stmt -> LogicType -> (IncLoLang.state) -> (IncLoLang.state) -> Prop
-| seq_er {S T s t u} (H1: post S LogicType.ok s t) (H2: post T LogicType.er t u) : /- TODO: This needs to use post norm instead? How to encode? -/
-  post (S ;; T) LogicType.er s u
-| error {s}:
-  post IncLoLang.stmt.error LogicType.er s s
+inductive lang_semantics: IncLoLang.stmt -> LogicType -> (IncLoLang.state) -> (IncLoLang.state) -> Prop
 | skip {s} :
-  post IncLoLang.stmt.skip LogicType.ok s s
+  lang_semantics IncLoLang.stmt.skip LogicType.ok s s
+| seq_ok {S T s t u} (H1: lang_semantics S LogicType.ok s t) (H2: lang_semantics T LogicType.ok t u) :
+  lang_semantics(S ;; T) LogicType.ok s u
+| seq_er {S T s t u} (H1: lang_semantics S LogicType.ok s t) (H2: lang_semantics T LogicType.er t u) : 
+  lang_semantics (S ;; T) LogicType.er s u
+| error {s}:
+  lang_semantics IncLoLang.stmt.error LogicType.er s s
 | assign {x s f} :
-  post (IncLoLang.stmt.assign x f) LogicType.ok s (s{x ↦ (f s)})
-| seq_ok {S T s t u} (H1: post S LogicType.ok s t) (H2: post T LogicType.ok t u) :
-  post(S ;; T) LogicType.ok s u
+  lang_semantics (IncLoLang.stmt.assign x f) LogicType.ok s (s{x ↦ (f s)})
 
-def incorrectness_logic (ty: LogicType) (P : (IncLoLang.state) → Prop) (R : IncLoLang.stmt)
-  (Q : (IncLoLang.state) → Prop) : Prop := 
-  ∀ s t, Q s -> post R ty t s -> P t
+def post (ty: LogicType) (r: IncLoLang.stmt) (P: IncLoLang.state -> Prop) : IncLoLang.state -> Prop 
+  := λ st, ∃ σ, P σ ∧ lang_semantics r ty σ st
 
-def hoare_logic (ty: LogicType) (P : (IncLoLang.state) → Prop) (R : IncLoLang.stmt)
+/- TODO: Change encoding of state-/
+/- state × ℕ -> prop -/
+
+def incorrectness_logic (type: LogicType) (P : (IncLoLang.state) → Prop) (R : IncLoLang.stmt)
   (Q : (IncLoLang.state) → Prop) : Prop := 
-  ∀ s t, P s -> post R ty t s -> Q t
+  ∀ state, Q state -> ((post type R) P) state
+
+def hoare_logic (type: LogicType) (P : (IncLoLang.state) → Prop) (R : IncLoLang.stmt)
+  (Q : (IncLoLang.state) → Prop) : Prop := 
+  ∀ state, ((post type R) P) state -> Q state
 
 notation `{* ` P : 1 ` *} ` S : 1 ` {* ` Q : 1 ` *}` ty: 2 :=
   hoare_logic ty P S Q
 
 notation `[* ` P : 1 ` *] ` S : 1 ` [* ` Q : 1 ` *]` ty: 2 :=
-  hoare_logic ty P S Q
+  incorrectness_logic ty P S Q
 
 lemma hoare_skip_intro_ok { P: IncLoLang.state -> Prop } : {* P *} IncLoLang.stmt.skip {* P *} LogicType.ok:=
 begin
-  intros s t hs hst,
-  cases hst,
-  assumption,
+  intros state h,
+
+  rcases h with ⟨σ, ⟨h₁, h₂⟩⟩,
+
+  cases h₂,
+  finish,
 end
 
-lemma hoare_skip_intro_er { P: IncLoLang.state -> Prop } : {* P *} IncLoLang.stmt.skip {* P *} LogicType.er :=
+lemma inc_skip_intro_er { P: IncLoLang.state -> Prop } : [* P *] IncLoLang.stmt.error [* P *] LogicType.er :=
 begin
-  intros s t hs hst,
-  cases hst,
+  intros state h,
+
+  use state,
+
+  split,
+  {finish,},
+  {
+    exact lang_semantics.error
+  },
 end
 
-
-lemma inc_skip_intro_ok { P: IncLoLang.state -> Prop } : [* P *] IncLoLang.stmt.skip [* P *] LogicType.ok:=
-begin
-  intros s t hs hst,
-  cases hst,
-  assumption,
-end
-
-lemma inc_skip_intro_er { P: IncLoLang.state -> Prop } : [* P *] IncLoLang.stmt.skip [* P *] LogicType.er :=
-begin
-  intros s t hs hst,
-  cases hst,
-end
+-- lemma seq_intro_hoare {P Q R S T} (hS : {* P *} S {* Q *} LogicType.ok)
+--     (hT : {* Q *} T {* R *} LogicType.ok) :
+--   {* P *} S ;; T {* R *} LogicType.ok :=
+-- begin
+--   intros s t hs hst,
+--   cases' hst,
+--   apply hT,
+--   { apply hS,
+--     { exact hs },
+--     { assumption } },
+--   { assumption }
+-- end
 
 end IncLoIncorrectness
