lean/language.lean
@@ -17,34 +17,18 @@ namespace IncLoLang
 
 meta def tactic.dec_trivial := `[exact dec_trivial]
 
-def state : Type := string -> ℕ
+def state : Type := string × ℕ -> Prop
 
 def state.update : string -> ℕ -> state -> state
-| name val s          := (λname', if name' = name then val else s name')
+| name val s := (λ pair, pair == (name, val) ∨ s pair)
 
 notation s `{` name ` ↦ ` val `}` := state.update name val s
 
 @[simp] lemma update_apply (name : string) (val : ℕ) (s : state) :
-  s{name ↦ val} name = val :=
+  s{name ↦ val} (name, val) :=
 begin
-  calc s{name ↦ val} name = (λname', if name' = name then val else s name') name : by refl
-       ...                = val : by finish,
-end
-
-@[simp] lemma update_apply_ne (name name' : string) (val : ℕ) (s : state) 
-  (h : name' ≠ name . tactic.dec_trivial) : 
-    s{name ↦ val} name' = s name' :=
-begin
-  calc s{name ↦ val} name' = (λname', if name' = name then val else s name') name' : by refl
-       ...                 = s name' : by finish[h],
-end
-
-@[simp] lemma update_override (name : string) (val₁ val₂ : ℕ) (s : state) :
-  s{name ↦ val₂}{name ↦ val₁} = s{name ↦ val₁} :=
-begin
-  apply funext,
-  intro name',
-  by_cases name' = name; simp [h]
+  unfold state.update,
+  finish,
 end
 
 /-! ## Language -/
@@ -57,25 +41,6 @@ inductive stmt : Type
 -- | ite    : (state → Prop) → stmt → stmt → stmt
 -- | while  : (state → Prop) → stmt → stmt
 
-def eval : option state -> stmt -> option state
-| st stmt.skip                  := st
-| none (stmt.assign v s)        := none
-| (some st) (stmt.assign v s)   := st{v ↦ s st}
-| st (stmt.seq n m)             := (eval (eval st n) m)
-| st (stmt.error)             := none
-
 infixr ` ;; ` : 90 := stmt.seq
-
-#eval option.bind (eval (some (λ x, 0)) stmt.skip) (λ s, some (s "x"))
-#eval option.bind (eval (some (λ x, if x = "y" then 2 else 0)) (stmt.assign "x" (λ s, 1 + s "y"))) 
-  (λ s, some (s "x"))
-#eval option.bind (eval (some (λ x, if x = "y" then 2 else 0))
-  ((stmt.assign "x" (λ s, 1 + s "y")) ;; 
-   (stmt.assign "x" (λ s, 1 + s "x")))) (λ s, some (s "x"))
-
-#eval option.bind (eval (none)
-  ((stmt.assign "x" (λ s, 1 + s "y")) ;; 
-   (stmt.assign "x" (λ s, 1 + s "x")))) (λ s, some (s "x"))
-#eval option.bind (eval (some (λ x, 0)) stmt.error) (λ s, some (s "x"))
 
 end IncLoLang
